Make stm_fail a valid final statement; work on automation
Add ResultOrFail predicate and use it in the statement of the program
logic soundness.

Work on Ltac automation for instantiating inductive hypothesises in the
program logic soundness proof

Finish rule_stm_match_sum case

src/MicroSail/Syntax.v
@@ -1147,6 +1147,19 @@ Module Terms (typekit : TypeKit) (termkit : TermKit typekit).
       | _ => False
       end.
 
+    Definition ResultOrFail {Γ σ} (s : Stm Γ σ) :
+      forall (POST : Lit σ -> Prop), Prop :=
+      match s with
+      | stm_lit _ v => fun POST => POST v
+      | stm_fail _ _ => fun _ => True
+      | _ => fun _ => False
+      end.
+
+    Lemma result_or_fail_inversion {Γ σ} (s : Stm Γ σ) (POST : Lit σ -> Prop) :
+      ResultOrFail s POST -> (exists msg, s = stm_fail _ msg)
+                          \/ (exists v, s = stm_lit _ v /\ POST v).
+    Proof. destruct s; cbn in *; try contradiction; eauto. Qed.
+
     (* This predicate encodes that the statement s is a finished computation and
        that the result is not a failure. This is a computational version that is
        better suited for the goal and the inversion below is better suited for
